Update the AES-GCM decryption impl to match the new spec

src/crypto/aes/GCM_i.fst
@@ -61,21 +61,63 @@ let gcm_encrypt_LE_snd_helper (iv_BE length_quad32 hash mac:quad32) (plain auth 
   //()
 
 
-let decrypt_helper (alg:algorithm) (key:aes_key alg) (iv:seqn 16 nat8) (plain:seq nat8) (auth:seq nat8)
+let lemma_gcm_encrypt_decrypt_equiv (alg:algorithm) (key:aes_key_LE alg) (iv_BE:quad32) (plain cipher auth alleged_tag:seq nat8) : Lemma
+  (requires 4096 * length cipher < pow2_32 /\
+            4096 * length auth < pow2_32 /\
+            plain == fst (gcm_encrypt_LE alg (seq_nat32_to_seq_nat8_LE key) (be_quad32_to_bytes iv_BE) cipher auth))
+  (ensures plain == fst (gcm_decrypt_LE alg (seq_nat32_to_seq_nat8_LE key) (be_quad32_to_bytes iv_BE) cipher auth alleged_tag))
+  =
+  reveal_opaque (gcm_encrypt_LE_def alg (seq_nat32_to_seq_nat8_LE key) (be_quad32_to_bytes iv_BE) cipher auth);
+  reveal_opaque (gcm_decrypt_LE_def alg (seq_nat32_to_seq_nat8_LE key) (be_quad32_to_bytes iv_BE) cipher auth alleged_tag);
+  ()
+  
+
+let gcm_decrypt_LE_tag (alg:algorithm) (key:aes_key alg) (iv:seqn 16 nat8) (cipher:seq nat8) (auth:seq nat8) :
+  Pure (seq nat8)
+    (requires
+      4096 * length cipher < pow2_32 /\
+      4096 * length auth < pow2_32
+    )
+    (ensures fun t -> True)
+  =
+  let key_LE = seq_nat8_to_seq_nat32_LE key in
+  let iv_BE = be_bytes_to_quad32 iv in
+  let h_LE = aes_encrypt_LE alg key_LE (Mkfour 0 0 0 0) in
+  let j0_BE = Mkfour 1 iv_BE.lo1 iv_BE.hi2 iv_BE.hi3 in
+
+  let lengths_BE = Mkfour (8 * length cipher) 0 (8 * length auth) 0 in
+  let lengths_LE = reverse_bytes_quad32 lengths_BE in
+
+  let zero_padded_c_LE = le_bytes_to_seq_quad32 (pad_to_128_bits cipher) in
+  let zero_padded_a_LE = le_bytes_to_seq_quad32 (pad_to_128_bits auth) in
+
+  let hash_input_LE = append zero_padded_a_LE (append zero_padded_c_LE (create 1 lengths_LE)) in
+  let s_LE = ghash_LE h_LE hash_input_LE in
+  let t = gctr_encrypt_LE j0_BE (le_quad32_to_bytes s_LE) alg key_LE in
+  t
+  
+  
+let decrypt_helper (alg:algorithm) (key:aes_key alg) (iv:seqn 16 nat8) (cipher:seq nat8) (auth:seq nat8)
                    (rax:nat64) (alleged_tag_quad computed_tag:quad32) : Lemma
-  (requires 4096 * length plain < pow2_32 /\
+  (requires 4096 * length cipher < pow2_32 /\
             4096 * length auth < pow2_32 /\
             (if alleged_tag_quad = computed_tag then rax = 0 else rax > 0) /\
-            le_quad32_to_bytes computed_tag == snd (gcm_encrypt_LE alg key iv plain auth)
+            le_quad32_to_bytes computed_tag == gcm_decrypt_LE_tag alg key iv cipher auth
   )
-  (ensures  (rax = 0) == snd (gcm_decrypt_LE alg key iv plain auth (le_quad32_to_bytes alleged_tag_quad)))
+  (ensures  (rax = 0) == snd (gcm_decrypt_LE alg key iv cipher auth (le_quad32_to_bytes alleged_tag_quad)))
   = 
-  let b = snd (gcm_decrypt_LE alg key iv plain auth (le_quad32_to_bytes alleged_tag_quad)) in
-  let (_, ct) = gcm_encrypt_LE alg key iv plain auth in
+  reveal_opaque (gcm_decrypt_LE_def alg key iv cipher auth (le_quad32_to_bytes alleged_tag_quad));
+  (*
+  let b = snd (gcm_decrypt_LE alg key iv cipher auth (le_quad32_to_bytes alleged_tag_quad)) in
+  let (_, ct) = gcm_decrypt_LE alg key iv cipher auth (le_quad32_to_bytes alleged_tag_quad) in
+
   assert (b = (ct = (le_quad32_to_bytes alleged_tag_quad)));
   assert (ct == le_quad32_to_bytes computed_tag);
   assert (b == (le_quad32_to_bytes computed_tag = le_quad32_to_bytes alleged_tag_quad));
+  *)
   le_quad32_to_bytes_injective_specific alleged_tag_quad computed_tag;
+  (*
   assert (b == (computed_tag = alleged_tag_quad));
   assert ((rax = 0) == (computed_tag = alleged_tag_quad));
+  *)
   ()
